VCVio.lean
@@ -13,8 +13,6 @@ import VCVio.CryptoFoundations.FiatShamir
 import VCVio.CryptoFoundations.FiatShamirWithAbort
 import VCVio.CryptoFoundations.Fischlin
 import VCVio.CryptoFoundations.Fork
-import VCVio.CryptoFoundations.ForkRuntime
-import VCVio.CryptoFoundations.ForkValues
 import VCVio.CryptoFoundations.FujisakiOkamoto.Composed
 import VCVio.CryptoFoundations.FujisakiOkamoto.Defs
 import VCVio.CryptoFoundations.FujisakiOkamoto.TTransform
@@ -31,7 +29,6 @@ import VCVio.CryptoFoundations.MacAlg
 import VCVio.CryptoFoundations.PRF
 import VCVio.CryptoFoundations.PRG
 import VCVio.CryptoFoundations.SecExp
-import VCVio.CryptoFoundations.SigmaExtractorRuntime
 import VCVio.CryptoFoundations.SigmaProtocol
 import VCVio.CryptoFoundations.SignatureAlg
 import VCVio.CryptoFoundations.SymmEncAlg
